Scott1980.lean
@@ -206,3 +206,6 @@ import Scott1980.Neighborhood.SplitV
 import Scott1980.Neighborhood.VDiff
 import Scott1980.Neighborhood.UBisection2
 import Scott1980.Neighborhood.Exercise812f
+import Scott1980.Neighborhood.Exercise812g1a
+import Scott1980.Neighborhood.Exercise812g1b
+import Scott1980.Neighborhood.Exercise812g2
